\newpage
\section*{Problem 2}

\subsection*{Question 2.1}
Refuting the validity of the formular, we negate the formular and try to find counter example.

The clausal form (CNF) of the formular is found:

\begin{center}
    \begin{tabular}{ clr }
        $\neg ((p \land q) \to (q \land p))$ & $\equiv \neg ((p \land q) \lor (q \land p))$ \\ 
        & $\equiv \neg ((\neg p \lor \neg q) \lor (q \land p))$ \\ 
        & $\equiv (\neg (\neg p \lor \neg q) \land \neg (q \land p))$ \\
        & $\equiv (\neg (\neg p \lor \neg q) \land (\neg q \lor \neg p))$ \\
        & $\equiv ( (\neg \neg p \land \neg \neg q) \land (\neg q \lor \neg p))$ \\
        & $\equiv p \land q \land (\neg q \lor \neg p)$
    \end{tabular}
\end{center}

The clauses are now clear and can be used in resolution:
\begin{center}
    \begin{tabular}{ clr }
        1. & $p$ & \\
        2. & $q$ & \\
        3. & $\bar{q}, \bar{p}$ & \\
        4. & $\bar{q}$ & 1,3 \\
        5. & $\square$ & 2,4 \\
    \end{tabular}
\end{center}

The empty clause $\square$ is derived, thus no interpretation of the original set of clauses can hold, it is unsatisfiable. 
As a result of refutation hence negation, the formular then holds in all interpretation. The formular is valid and therefor a tautology.

\subsection*{Question 2.2}
Refuting the validity of the formular, we negate the formular and try to find counter example:

\Tree[.\textit{$\neg ((\forall x \exists y (p(x) \land \neg p(y))) \to \neg q(a))$} 
        [ .\textit{$\forall x \exists y (p(x) \land \neg p(y)), \neg \neg q(a)$} 
            [.\textit{$ \forall x \exists y (p(x) \land \neg p(y)), q(a) $}
                [.\textit{$\forall x \exists y (p(x) \land \neg p(y)) ,\exists y (p(a) \land \neg p(y)), q(a)$} 
                    [.\textit{$\forall x \exists y (p(x) \land \neg p(y)) ,p(a) \land \neg p(b), q(a)$}
                        [.\textit{$\forall x \exists y (p(x) \land \neg p(y)) , p(a) , \neg p(b), q(a)$} 
                            [.\textit{$\forall x \exists y (p(x) \land \neg p(y)), \exists y (p(b) \land \neg p(y)) , p(a) , \neg p(b), q(a)$} 
                                [.\textit{$\forall x \exists y (p(x) \land \neg p(y)), p(b) \land \neg p(c) , p(a) , \neg p(b), q(a)$} 
                                    [.\textit{$\forall x \exists y (p(x) \land \neg p(y)), p(b) , \neg p(c) , p(a) , \neg p(b), q(a)$} 
                                        \textit{$\times$}
                                    ] 
                                ] 
                            ] 
                        ] 
                    ] 
                ] 
            ]
        ]
]

The tableau closes as we see the contradiction with: $p(b)$ and $\neg p(b)$.
This concludes a complete closed tableau, thus we can say that the formula is valid. Because we negated the formular, the contradiction becomes a tautology.
