\newpage
\section*{Problem 2}

\subsection*{Question 2.1}
Refuting the validity of the expression, we negate it and try to find counter example:

\Tree[.\textit{$\neg (((s \to p) \land ((\neg s \to t) \land (\neg p \to \neg t))) \to p)$} 
        [ .\textit{$\neg ((s \to p) \land ((\neg s \to t) \land (\neg p \to \neg t))) , \neg p$} 
            [.\textit{$\neg (s \to p), \neg p$}
                [.\textit{$\neg s, \neg p, \neg p$} \textit{$\odot$} ] ]
            [.\textit{$\neg ((\neg s \to t) \land (\neg p \to \neg t)), \neg p$} 
                [.\textit{$\neg (\neg s \to t), \neg p$} 
                    [.\textit{$\neg s , \neg t, \neg p$} \textit{$\odot$} ]
                ]
                [.\textit{$\neg (\neg p \to \neg t), \neg p$} 
                    [.\textit{$\neg p , t, \neg p$} \textit{$\odot$} ]
                ]
            ]    
        ]
    ]


From the first right branch, we can see that the expression is not valid. As if s is true,
Watch week 4 solutions for inspiration about refutionation blabla

\subsection*{Question 2.2}
Brug den logiske regl p√• udtrykket og se det giver mening:

\subsection*{Question 2.3}